some disjointness and cover lemmas

src/functional.lean
@@ -3,6 +3,7 @@
 --import .variability
 import data.fintype
 import data.finset
+import tactic.basic
 
 namespace functional
 
@@ -10,7 +11,7 @@ variables {α β : Type}
 
 section func
 
-inductive PC (Feature : Type) : Type
+inductive PC {Feature : Type} : Type
 | All  : PC 
 | None : PC
 | Atom : Feature → PC 
@@ -28,35 +29,141 @@ def allConfigs (Feature : Type) [fintype Feature]
 
 open PC
 
+--@[simp]
 def semantics {Feature : Type} [fintype Feature] [decidable_eq Feature]
-    : PC Feature → finset (finset Feature)
-| (All Feature) := allConfigs Feature
-| (None Feature):= ∅
+    : PC → finset (finset Feature)
+| (All) := allConfigs Feature
+| (None):= ∅
 | (Atom f)      := (allConfigs Feature).filter (λ p, f ∈ p)
 | (Not pc)      := (allConfigs Feature).filter (λ p, p ∈ (semantics pc))
 | (And pc₁ pc₂) := (semantics pc₁) ∩ (semantics pc₂)
 | (Or  pc₁ pc₂) := (semantics pc₁) ∪ (semantics pc₂)
 
 structure Var {Feature: Type} [fintype Feature] (α : Type) := 
-    (v : α) (pc : PC Feature)
+    (v : α) (pc : @PC Feature)
+
+--@[simp]
+def disjoint {Feature : Type} [fintype Feature] [decidable_eq Feature]
+    (pc₁ : @PC Feature) (pc₂ : PC) : Prop :=
+    semantics (And pc₁ pc₂) = ∅ 
+
+lemma conj_preserves_disjoint {Feature : Type} [fintype Feature] [decidable_eq Feature] :
+    ∀ (pc₁ : @PC Feature) (pc₂ : PC) (c : PC), disjoint pc₁ pc₂ → disjoint (And c pc₁) (And c pc₂) :=
+    begin 
+        --simp,   -- ∀ (pc₁ pc₂ c : PC), semantics (And pc₁ pc₂) = ∅ → 
+                -- semantics (And (And c pc₁) (And c pc₂)) = ∅ 
+        intros, -- semantics (And (And c pc₁) (And c pc₂)) = ∅
+        unfold disjoint, unfold disjoint at a,
+        unfold semantics, -- semantics c ∩ semantics pc₁ ∩ (semantics c ∩ semantics pc₂) = ∅
+        unfold semantics at a, -- a : semantics pc₁ ∩ semantics pc₂ = ∅ 
+        simp, 
+        rw← finset.inter_assoc,
+        rw a, -- ∅ ∩ semantics c = ∅ 
+        apply finset.empty_inter
+    end
+
+--@[simp]
+def disjointList {Feature : Type} [t : fintype Feature] [decidable_eq Feature] {α : Type}
+    (vs : list (@Var Feature t α)) : Prop :=
+    ∀ (x y : Var α) , x ∈ vs → y ∈ vs → x.pc ≠ y.pc → disjoint x.pc y.pc
+
+def cover {Feature : Type} [t : fintype Feature] [d : decidable_eq Feature] {α : Type}
+    (v : list (@Var Feature t α)) := 
+    semantics(list.foldr Or None (list.map (Var.pc) v))
 
 structure Lifted {Feature: Type} [fintype Feature] [decidable_eq Feature] (α : Type) := 
     (s : list (Var α))
-    (disjoint : ∀ p q : Var α, p ∈ s ∧ q ∈ s ∧ p ≠ q → (semantics (And p.pc q.pc)) = ∅)
-    (complete : semantics(list.foldr Or (None Feature) (list.map (Var.pc) s)) = allConfigs Feature)
+    (disj : disjointList s)
+    (comp : cover s = allConfigs Feature)
 
 notation `⟦` p `⟧` := (semantics p)
 postfix `↑`:(max+1) := Lifted
 
-def apply_inner {Feature : Type} [t: fintype Feature] [d: decidable_eq Feature] 
+--@[simp]
+def apply_single {Feature : Type} [t: fintype Feature] [d: decidable_eq Feature] 
     (f : @Var Feature t (α → β)) (u : α↑) : list (@Var Feature t β) :=
     let sat := list.filter (λ(v : Var α), ⟦And f.pc v.pc⟧ ≠ ∅) u.s in
     list.map (λ(v':Var α), Var.mk (f.v v'.v) (And f.pc  v'.pc)) sat
+ 
+lemma apply_single_disj {Feature : Type} [t: fintype Feature] [d: decidable_eq Feature] {α β : Type} : 
+    ∀ (f : @Var Feature t (α → β)) (u : @Lifted Feature t d α), disjointList (apply_single f u) :=
+begin
+    unfold apply_single, simp,
+    intros, unfold disjointList, simp, intros, 
+    rw[←a_2,←a_5], simp, apply conj_preserves_disjoint,
+    apply u.disj, apply a, apply a_3,
+    rw [←a_2, ←a_5] at a_6, simp at a_6, apply a_6
+end
+
+section 
+open classical
+
+lemma apply_single_cover {Feature : Type} [t : fintype Feature] [d: decidable_eq Feature] {α β : Type} :
+    ∀ (f : @Var Feature t (α → β)) (u : @Lifted Feature t d α),
+    cover (apply_single f u) = ⟦f.pc⟧ ∩ cover u.s :=
+begin
+    intros, unfold apply_single, 
+    induction u.s,
+    -- base case
+    simp, unfold cover, simp, unfold semantics, simp, 
+    -- induction
+    simp, unfold list.filter,  
+    --unfold cover, simp,
+    -- we need excluded middle.. this will be a classical proof
+    cases decidable.em (semantics (PC.And (f.pc) (hd.pc)) = ∅) with hEmpty hNEmpty, 
+    {
+        rw← hEmpty, simp, rw hEmpty, simp at ih, rw ih, unfold cover, simp,
+        unfold semantics, rw finset.inter_distrib_left, unfold semantics at hEmpty, 
+        rw hEmpty, rw finset.empty_union   
+    },
+    {
+        rw (if_pos hNEmpty), simp at ih, simp, unfold cover, simp, unfold cover at ih, 
+        unfold semantics, unfold semantics at ih, simp at ih, simp, rw ih,
+        rw finset.inter_distrib_left, simp     
+    }
+    
+end -- section
+#print 
+
+lemma apply_single_append {Feature : Type} [t : fintype Feature] [d: decidable_eq Feature] {α β : Type} :
+    ∀ (f₁ f₂ : @Var Feature t (α → β)) (u : @Lifted Feature t d α),
+    disjoint f₁.pc f₂.pc → disjointList (apply_single f₁ u) → disjointList (apply_single f₂ u) →
+    disjointList (list.append (apply_single f₁ u) (apply_single f₂ u)) :=
+begin
+    intros f₁ f₂ u,
+    generalize : (apply_single f₁ u) = l₁,
+    intros h₁ h₂ h₃,  
+    induction l₁,
+    -- base case
+    simp, apply h₃, 
+    -- induction
+    simp, unfold disjointList at h₂, 
+end
+
+@[simp]
+def apply_inner {Feature : Type} [t: fintype Feature] [d: decidable_eq Feature] 
+    (f : @Lifted Feature t d (α → β)) (v : @Lifted Feature t d α) : list (@Var Feature t β) :=
+    list.foldr list.append [] (list.map (λ x, apply_single x v) f.s
+
+lemma apply_inner_disjoint {Feature : Type} [t: fintype Feature] [d: decidable_eq Feature] {α β : Type} : 
+    ∀ (f : @Lifted Feature t d (α → β)) (v : @Lifted Feature t d α),
+    disjointList(apply_inner f v) :=
+begin
+    unfold apply_inner, intros, induction f.s, 
+    -- base case
+    unfold disjointList, simp,
+    -- induction step  
+    unfold list.map, unfold list.foldr, 
+    unfold disjointList, intros, 
+end
+
 
 def apply {Feature : Type} [t: fintype Feature] [d: decidable_eq Feature] 
     (f : @Lifted Feature t d (α → β)) (v : @Lifted Feature t d α) : @Lifted Feature t d β :=
-    ⟨list.foldr list.append [] (list.map (λ x, apply_inner x v) f.s),
-    _,
+    ⟨apply_inner f v,
+    begin 
+        intros, simp, intros, 
+    end,
     _⟩
 
 end func
